protobuf-shim/proofs/fstar/extraction/Protobuf.Enum_or_unknown.fsti
@@ -9,18 +9,26 @@ let _ =
   let open Protobuf.Enums in
   ()
 
-let impl___HAX_PLACEHOLDER (#v_E: Type0) : Prims.unit = () <: Prims.unit
+let impl___HAX_PLACEHOLDER
+      (#v_E: Type0)
+      (#[FStar.Tactics.Typeclasses.tcresolve ()] i1: Core.Clone.t_Clone v_E)
+    : Prims.unit = () <: Prims.unit
 
-type t_EnumOrUnknown (v_E: Type0) = {
+type t_EnumOrUnknown (v_E: Type0) {| i1: Core.Clone.t_Clone v_E |} = {
   f_value:i32;
   f_phantom:Core.Marker.t_PhantomData v_E
 }
 
-val impl_1__enum_value (#v_E: Type0) {| i1: Protobuf.Enums.t_Enum v_E |} (self: t_EnumOrUnknown v_E)
+val impl_1__enum_value
+      (#v_E: Type0)
+      {| i1: Protobuf.Enums.t_Enum v_E |}
+      {| i2: Core.Clone.t_Clone v_E |}
+      (self: t_EnumOrUnknown v_E)
     : Prims.Pure (Core.Result.t_Result v_E i32) Prims.l_True (fun _ -> Prims.l_True)
 
 val impl_1__enum_value_or_default
       (#v_E: Type0)
-      {| i2: Protobuf.Enums.t_Enum v_E |}
+      {| i3: Protobuf.Enums.t_Enum v_E |}
+      {| i3: Core.Clone.t_Clone v_E |}
       (self: t_EnumOrUnknown v_E)
     : Prims.Pure v_E Prims.l_True (fun _ -> Prims.l_True)
