protobuf-shim/proofs/fstar/extraction/Protobuf.Message_field.fst
@@ -3,7 +3,11 @@ module Protobuf.Message_field
 open Core
 open FStar.Mul
 
-let impl__as_ref (#v_T: Type0) (self: t_MessageField v_T) =
+let impl__as_ref
+      (#v_T: Type0)
+      (#[FStar.Tactics.Typeclasses.tcresolve ()] i1: Core.Clone.t_Clone v_T)
+      (self: t_MessageField v_T)
+     =
   Core.Option.impl__map #(Alloc.Boxed.t_Box v_T Alloc.Alloc.t_Global)
     #v_T
     (Core.Option.impl__as_ref #(Alloc.Boxed.t_Box v_T Alloc.Alloc.t_Global) self._0
@@ -11,5 +15,8 @@ let impl__as_ref (#v_T: Type0) (self: t_MessageField v_T) =
       Core.Option.t_Option (Alloc.Boxed.t_Box v_T Alloc.Alloc.t_Global))
     (fun v -> v)
 
-let impl__is_some (#v_T: Type0) (self: t_MessageField v_T) =
-  Core.Option.impl__is_some #(Alloc.Boxed.t_Box v_T Alloc.Alloc.t_Global) self._0
+let impl__is_some
+      (#v_T: Type0)
+      (#[FStar.Tactics.Typeclasses.tcresolve ()] i2: Core.Clone.t_Clone v_T)
+      (self: t_MessageField v_T)
+     = Core.Option.impl__is_some #(Alloc.Boxed.t_Box v_T Alloc.Alloc.t_Global) self._0
