protobuf-shim/proofs/fstar/extraction/Protobuf.Message_field.fsti
@@ -3,12 +3,12 @@ module Protobuf.Message_field
 open Core
 open FStar.Mul
 
-type t_MessageField (v_T: Type0) =
+type t_MessageField (v_T: Type0) {| i1: Core.Clone.t_Clone v_T |} =
   | MessageField : Core.Option.t_Option (Alloc.Boxed.t_Box v_T Alloc.Alloc.t_Global)
     -> t_MessageField v_T
 
-val impl__as_ref (#v_T: Type0) (self: t_MessageField v_T)
+val impl__as_ref (#v_T: Type0) {| i1: Core.Clone.t_Clone v_T |} (self: t_MessageField v_T)
     : Prims.Pure (Core.Option.t_Option v_T) Prims.l_True (fun _ -> Prims.l_True)
 
-val impl__is_some (#v_T: Type0) (self: t_MessageField v_T)
+val impl__is_some (#v_T: Type0) {| i2: Core.Clone.t_Clone v_T |} (self: t_MessageField v_T)
     : Prims.Pure bool Prims.l_True (fun _ -> Prims.l_True)
