protobuf-shim/proofs/fstar/extraction/Protobuf.Reflect.File.fsti
@@ -3,4 +3,24 @@ module Protobuf.Reflect.File
 open Core
 open FStar.Mul
 
-type t_FileDescriptor = { f__hax_placeholder:Prims.unit }
+type t_DynamicFileDescriptor = {
+  f_proto:Protobuf.Descriptor.t_FileDescriptorProto;
+  f_common:Protobuf.Reflect.File.Index.t_FileDescriptorCommon
+}
+
+type t_FileDescriptorImpl =
+  | FileDescriptorImpl_Generated : Protobuf.Reflect.File.Generated.t_GeneratedFileDescriptor
+    -> t_FileDescriptorImpl
+  | FileDescriptorImpl_Dynamic : t_DynamicFileDescriptor -> t_FileDescriptorImpl
+
+type t_FileDescriptor = { f_imp:t_FileDescriptorImpl }
+
+val impl__FileDescriptor__common (self: t_FileDescriptor)
+    : Prims.Pure Protobuf.Reflect.File.Index.t_FileDescriptorCommon
+      Prims.l_True
+      (fun _ -> Prims.l_True)
+
+val impl__FileDescriptor__enum_by_package_relative_name (self: t_FileDescriptor) (name: string)
+    : Prims.Pure (Core.Option.t_Option Protobuf.Reflect.Enums.t_EnumDescriptor)
+      Prims.l_True
+      (fun _ -> Prims.l_True)
