protobuf-shim/proofs/fstar/extraction/Protobuf.Reflect.Enums.fst
@@ -1,0 +1,7 @@
+module Protobuf.Reflect.Enums
+#set-options "--fuel 0 --ifuel 1 --z3rlimit 15"
+open Core
+open FStar.Mul
+
+let impl__EnumDescriptor__new (#v_T: Type0) (file_descriptor: v_T) (index: usize) =
+  { f__hax_placeholder = () <: Prims.unit } <: t_EnumDescriptor
