protobuf-shim/proofs/fstar/extraction/Protobuf.Reflect.Enums.fsti
@@ -4,3 +4,6 @@ open Core
 open FStar.Mul
 
 type t_EnumDescriptor = { f__hax_placeholder:Prims.unit }
+
+val impl__EnumDescriptor__new (#v_T: Type0) (file_descriptor: v_T) (index: usize)
+    : Prims.Pure t_EnumDescriptor Prims.l_True (fun _ -> Prims.l_True)
