protobuf-shim/proofs/fstar/extraction/Protobuf.Reflect.File.Generated.fsti
@@ -1,0 +1,6 @@
+module Protobuf.Reflect.File.Generated
+#set-options "--fuel 0 --ifuel 1 --z3rlimit 15"
+open Core
+open FStar.Mul
+
+type t_GeneratedFileDescriptor = { f_common:Protobuf.Reflect.File.Index.t_FileDescriptorCommon }
