protobuf-shim/proofs/fstar/extraction/Protobuf.Reflect.File.Index.fsti
@@ -1,0 +1,10 @@
+module Protobuf.Reflect.File.Index
+#set-options "--fuel 0 --ifuel 1 --z3rlimit 15"
+open Core
+open FStar.Mul
+
+type t_FileDescriptorCommon = {
+  f_enums_by_name_to_package:Std.Collections.Hash.Map.t_HashMap Alloc.String.t_String
+    usize
+    Std.Hash.Random.t_RandomState
+}
