protobuf-shim/proofs/fstar/extraction/Protobuf.Reflect.File.fst
@@ -1,0 +1,31 @@
+module Protobuf.Reflect.File
+#set-options "--fuel 0 --ifuel 1 --z3rlimit 15"
+open Core
+open FStar.Mul
+
+let impl__FileDescriptor__common (self: t_FileDescriptor) =
+  match self.f_imp with
+  | FileDescriptorImpl_Generated g -> g.Protobuf.Reflect.File.Generated.f_common
+  | FileDescriptorImpl_Dynamic d -> d.f_common
+
+let impl__FileDescriptor__enum_by_package_relative_name (self: t_FileDescriptor) (name: string) =
+  Core.Option.impl__map #usize
+    #Protobuf.Reflect.Enums.t_EnumDescriptor
+    (Std.Collections.Hash.Map.impl_2__get #Alloc.String.t_String
+        #usize
+        #Std.Hash.Random.t_RandomState
+        #string
+        (impl__FileDescriptor__common self <: Protobuf.Reflect.File.Index.t_FileDescriptorCommon)
+          .Protobuf.Reflect.File.Index.f_enums_by_name_to_package
+        name
+      <:
+      Core.Option.t_Option usize)
+    (fun index ->
+        let index:usize = index in
+        Protobuf.Reflect.Enums.impl__EnumDescriptor__new #t_FileDescriptor
+          (Core.Clone.f_clone #t_FileDescriptor #FStar.Tactics.Typeclasses.solve self
+            <:
+            t_FileDescriptor)
+          index
+        <:
+        Protobuf.Reflect.Enums.t_EnumDescriptor)
