protobuf-shim/proofs/fstar/extraction/Protobuf.Reflect.fsti
@@ -18,8 +18,6 @@ type t_MessageDescriptor = { f__hax_placeholder:Prims.unit }
 
 type t_OneofDescriptor = { f__hax_placeholder:Prims.unit }
 
-type t_SpecialFields = { f__hax_placeholder:Prims.unit }
-
 type t_Kind =
   | Kind_NullValue : Protobuf.Enum_or_unknown.t_EnumOrUnknown t_NullValue -> t_Kind
   | Kind_NumberValue : u64 -> t_Kind
@@ -30,17 +28,17 @@ type t_Kind =
 
 and t_ListValue = {
   f_values:Alloc.Vec.t_Vec t_Value Alloc.Alloc.t_Global;
-  f_special_fields:t_SpecialFields
+  f_special_fields:Protobuf.Special.t_SpecialFields
 }
 
 and t_Struct = {
   f_fields:Std.Collections.Hash.Map.t_HashMap Alloc.String.t_String
     t_Value
     Std.Hash.Random.t_RandomState;
-  f_special_fields:t_SpecialFields
+  f_special_fields:Protobuf.Special.t_SpecialFields
 }
 
 and t_Value = {
   f_kind:Core.Option.t_Option t_Kind;
-  f_special_fields:t_SpecialFields
+  f_special_fields:Protobuf.Special.t_SpecialFields
 }
